proof: labeling

policy_proof/coq/security.v
@@ -8,16 +8,15 @@ Require Import types.
 Fixpoint env_ok s (e : env s) : Prop :=
   match e with
     | nil => True
-    | (x, t) :: e' =>  False \/ env_ok _ e'
+    | (x, t) :: e' =>  False ∨ env_ok _ e'
   end.
 
 (* todo *)
 Theorem secure_query:
-  ∀ s ctx priv e o c,
+  ∀ s s' ctx ctx' priv priv' e e' o c,
     config_ok s ctx priv e =[ o ]=> c →
-      c = config_error \/
-      ∃ s' ctx' priv' e',
-        c = config_ok s' ctx' priv' e' /\ env_ok s' e'.
+      c = config_error ∨
+      c = config_ok s' ctx' priv' e' ∧ env_ok s' e'.
 Proof.
   intros.
 Admitted.
